Notiamo che se $(A\times Y)\cup (X\times B)=int(A\times Y)\cup int(X\times B)$ allora per quanto sappiamo sulle [[1&3 -Catene U-piccole|catene U-piccole]] si ha che $C_\bullet(A\times Y)+C_\bullet(X\times B)=C_\bullet^\Uc(A\times Y\cup X\times B)$, dunque per [[3-Eilenberg-Zilber|Eilenberg-Zilber]]$$H_\bullet(X\times Y,A\times Y\cup X\times B)=H_\bullet^\Uc(X\times Y,A\times Y\cup X\times B)\cong H_\bullet(C_\bullet(X,A)\otimes C_\bullet(Y,B)).$$Ha dunque senso porre $H_\bullet((X,A)\times (Y,B))=H_\bullet(X\times Y,A\times Y\cup X\times B)$.